doc/roadmap/v0-contracts-missing-proofs.md
@@ -1,0 +1,40 @@
+# Missing proofs
+## High
+
+High-priority proofs related to translation correctness
+
+### Pipit.Exp.Causality (base)
+prove lemma-bigstep-total
+
+### Pipit.System.Exp (trans)
+no translation for free vars: just treat them as oracles
+
+### Pipit.System.Exp.Properties (trans)
+translation is an abstraction (big)
+
+### Pipit.Prim.Table (base, easy)
+simple context proofs
+
+
+## Mid
+
+Medium-priority proofs related to preservation of checks
+
+### Pipit.Exp.Checked.Base (checks)
+bless proofs
+
+### Pipit.Sugar.Check (checks)
+induction is sound (big)
+
+### Pipit.System.Ind (checks)
+induction is sound, checks are preserved
+
+## Low
+
+Low-priority proofs: mainly just annoying
+
+### Pipit.Exp.Checked.Compound (checks, sugar)
+compounds preserve check
+
+### Pipit.Exp.Binding.Property (base)
+FLAKY
